deleted old definitions

src/miller_ssv.lean
@@ -24,7 +24,7 @@ def best_margin {χ υ : Type*} (voters : finset υ) (s : finset (χ × χ)) (Q 
     then s.sup' hn (λ p, margin voters Q p.1 p.2) 
   else 0
 
-def simple_stable_voting'' {χ υ : Type*} (voters : finset υ) (Q : υ → χ → χ → Prop)
+def simple_stable_voting' {χ υ : Type*} (voters : finset υ) (Q : υ → χ → χ → Prop)
   [decidable_eq χ] 
   [∀ v, decidable_rel (Q v)] :
   Π (n : ℕ) (candidates : finset χ) (hn : candidates.card = n) (cpos : 0 < n), finset χ
@@ -35,7 +35,7 @@ let
   -- whether c wins when candidate rem is removed
   still_wins (c rem : χ) : Prop :=
     if rem_prop : rem ∈ cands 
-      then c ∈ simple_stable_voting'' (n+1) (cands.erase rem)
+      then c ∈ simple_stable_voting' (n+1) (cands.erase rem)
           (by { rw [finset.card_erase_of_mem, hn]; simp [rem_prop], })
           (by omega)
     else false,
@@ -43,41 +43,14 @@ let
       (λ p, /-p.2 ∈ cands ∧ -/ still_wins p.1 p.2 )
 in finset.image prod.fst $ viable.filter (λ p, (margin voters Q p.1 p.2 = best_margin voters viable Q))
 
-def simple_stable_voting' {χ υ : Type*} (voters : finset υ) (Q : υ → χ → χ → Prop)
-  [decidable_eq χ] 
-  [∀ v, decidable_rel (Q v)] :
-  Π (n : ℕ) (candidates : finset χ) (hn : candidates.card = n) (cpos : 0 < n), finset χ
-| 0 _ _ cpos := (nat.not_lt_zero _ cpos).elim
-| 1 candidates _ _ := candidates
-| (n+2) cands hn cpos :=
-let
-  -- whether c wins when candidate rem is removed
-  still_wins (c rem : χ) (rem_prop : rem ∈ cands) : Prop :=
-    c ∈ simple_stable_voting' (n+1) (cands.erase rem)
-          (by { rw [finset.card_erase_of_mem, hn]; simp [rem_prop], })
-          (by omega),
-  viable : finset (χ × χ) := finset.image coe $
-    (cands.product cands).attach.filter (λ (p : cands.product cands),
-      still_wins p.1.1 p.1.2 (by { cases p, simp at p_property, exact p_property.2, }))
-in finset.image prod.fst $ viable.filter (λ p, (margin voters Q p.1 p.2 = best_margin voters viable Q))
-
 def simple_stable_voting {χ υ : Type*} (prof : election_profile χ υ)
   [decidable_eq χ] [∀ v, decidable_rel (prof.Q v)] : finset χ :=
 simple_stable_voting' prof.voters prof.Q prof.candidates.card prof.candidates rfl prof.cpos
-
-def simple_stable_voting_new {χ υ : Type*} (prof : election_profile χ υ)
-  [decidable_eq χ] [∀ v, decidable_rel (prof.Q v)] : finset χ :=
-simple_stable_voting'' prof.voters prof.Q prof.candidates.card prof.candidates rfl prof.cpos
 
 lemma ssv_singleton {χ υ : Type*} (prof : election_profile χ υ) (hcands : prof.candidates.card = 1)
   [decidable_eq χ] [∀ v, decidable_rel (prof.Q v)] : 
   simple_stable_voting prof = prof.candidates :=
 by simp only [simple_stable_voting, simple_stable_voting', hcands]
-
-lemma ssv_singleton_new {χ υ : Type*} (prof : election_profile χ υ) (hcands : prof.candidates.card = 1)
-  [decidable_eq χ] [∀ v, decidable_rel (prof.Q v)] : 
-  simple_stable_voting_new prof = prof.candidates :=
-by simp only [simple_stable_voting_new, simple_stable_voting'', hcands]
 
 lemma exists_best_margin {χ υ : Type*} {s : finset (χ × χ)} (voters : finset υ) (Q : υ → χ → χ → Prop) 
   [∀ v, decidable_rel (Q v)] (hs : s.nonempty) :
@@ -99,7 +72,7 @@ begin
   use d,
 end
 
-lemma mem_cands_of_mem_winners  {χ υ : Type*} (prof : election_profile χ υ) (a : χ)
+lemma mem_cands_of_mem_winners {χ υ : Type*} (prof : election_profile χ υ) (a : χ)
   [decidable_eq χ] [∀ v, decidable_rel (prof.Q v)] : 
   a ∈ simple_stable_voting prof → a ∈ prof.candidates := 
 begin
@@ -107,24 +80,7 @@ begin
   by_cases hcands : prof.candidates.card = 1, 
   { rwa ssv_singleton prof hcands at a_in, },
   obtain ⟨n, hn⟩ := exists_eq_plus_two prof.candidates.card (by linarith [prof.cpos]) hcands, 
-  simp only [simple_stable_voting, simple_stable_voting', hn, true_and, finset.mem_attach, 
-    exists_prop, exists_and_distrib_right, prod.mk.inj_iff, 
-    exists_eq_right_right, exists_eq_right, finset.mem_image, subtype.exists, finset.mem_filter,
-    finset.filter_congr_decidable, subtype.coe_mk, 
-    subtype.val_eq_coe, prod.exists, finset.mem_product] at a_in,
-  rcases a_in with ⟨b,⟨⟨p_in,hp⟩,ha⟩⟩,
-  exact (finset.mem_product.1 p_in).1,
-end
-
-lemma mem_cands_of_mem_winners_new  {χ υ : Type*} (prof : election_profile χ υ) (a : χ)
-  [decidable_eq χ] [∀ v, decidable_rel (prof.Q v)] : 
-  a ∈ simple_stable_voting_new prof → a ∈ prof.candidates := 
-begin
-  intro a_in,
-  by_cases hcands : prof.candidates.card = 1, 
-  { rwa ssv_singleton_new prof hcands at a_in, },
-  obtain ⟨n, hn⟩ := exists_eq_plus_two prof.candidates.card (by linarith [prof.cpos]) hcands, 
-  simp only [simple_stable_voting_new, simple_stable_voting'', hn, 
+  simp only [simple_stable_voting, simple_stable_voting', hn, 
     exists_prop, exists_and_distrib_right, exists_eq_right,
     finset.mem_image, finset.mem_filter, finset.filter_congr_decidable, 
     prod.exists, finset.mem_product] at a_in,
@@ -147,59 +103,6 @@ begin
   intros prof hm,
   set m := d.succ with m_succ,
   obtain ⟨b, b_in⟩ := finset.card_pos.1 prof.cpos,
-  have h_erase_b : finset.card (prof.candidates.erase b) = m,
-    { rw finset.card_erase_of_mem b_in,
-      exact nat.pred_eq_of_eq_succ hm, },
-  set prof' : election_profile χ υ := 
-    ⟨(prof.candidates.erase b), 
-     (by rw h_erase_b; omega), 
-     prof.voters, prof.vpos, prof.Q⟩ with h_prof',
-  have prof'_cands : prof'.candidates.card = m := by rw ← h_erase_b, 
-  obtain ⟨a, a_in⟩ := IH prof' prof'_cands,
-  have card_eq_d : prof.candidates.card = d + 2 := sorry, 
-  simp only [simple_stable_voting, simple_stable_voting', card_eq_d, true_and, 
-    finset.mem_attach, exists_prop,
-    exists_and_distrib_right, prod.mk.inj_iff, exists_eq_right_right, 
-    exists_eq_right, finset.mem_image, subtype.exists,
-    finset.mem_filter, finset.filter_congr_decidable, subtype.coe_mk, 
-    subtype.val_eq_coe, prod.exists, finset.mem_product],
-  
-  set viable_set : finset (χ × χ) := (prof.candidates.product prof.candidates).filter
-    (λ p, p.1 ∈ simple_stable_voting' prof.voters prof.Q d.succ (prof.candidates.erase p.2) sorry (nat.succ_pos d))
-    with hvs,
-  have viable_nonempty : viable_set.nonempty,
-  { use ⟨a,b⟩,
-    have : a ∈ (prof.candidates.erase b) := 
-      by simp only [mem_cands_of_mem_winners prof' a a_in],
-    simp only [finset.mem_filter, finset.mem_product],
-    simp only [simple_stable_voting, h_prof', h_erase_b, m_succ] at a_in,
-    refine ⟨⟨(finset.mem_erase.1 this).2, b_in⟩, a_in⟩, },  
-  obtain ⟨p, p_in, hp⟩ := exists_best_margin prof.voters prof.Q viable_nonempty,
-  refine ⟨p.1, p.2, ⟨_,_⟩⟩,
-  { rw hvs at p_in,
-    simp only [finset.mem_filter] at p_in,
-    split, {exact p_in.2, },
-    simp only [p_in.left, prod.mk.eta], },
-  { convert hp,
-    rw hvs,
-    sorry, },
-end
-
-lemma exists_ssv_winner'_new {χ υ : Type*} :
-  ∀ (n : ℕ) (prof : election_profile χ υ), prof.candidates.card = n → 
-  ∃ a, a ∈ simple_stable_voting_new prof :=
-begin
-  intro n,
-  cases n with d, 
-  { intros prof hn,
-    linarith [hn, prof.cpos], },
-  induction d with d IH,
-  { intros prof hn,
-    rw ssv_singleton_new prof hn,
-    exact finset.card_pos.1 prof.cpos, },
-  intros prof hm,
-  set m := d.succ with m_succ,
-  obtain ⟨b, b_in⟩ := finset.card_pos.1 prof.cpos,
   have h_erase_card : ∀ z ∈ prof.candidates, finset.card (prof.candidates.erase z) = m,
     { intros z z_in,
       rw finset.card_erase_of_mem z_in,
@@ -211,21 +114,21 @@ begin
   have prof'_cands : prof'.candidates.card = m := by rw ← h_erase_card b b_in, 
   obtain ⟨a, a_in⟩ := IH prof' prof'_cands,
   have card_eq_d : prof.candidates.card = d + 2 := by rw hm,
-  simp only [simple_stable_voting_new, simple_stable_voting'', card_eq_d, 
+  simp only [simple_stable_voting, simple_stable_voting', card_eq_d, 
     exists_prop, exists_and_distrib_right, exists_eq_right,
     finset.mem_image, finset.mem_filter, finset.filter_congr_decidable,
     prod.exists, finset.mem_product],
   set viable_set : finset (χ × χ) := (prof.candidates.product prof.candidates).filter
     (λ p, if p2_in : p.2 ∈ prof.candidates 
-      then p.1 ∈ simple_stable_voting'' prof.voters prof.Q d.succ (prof.candidates.erase p.2)
+      then p.1 ∈ simple_stable_voting' prof.voters prof.Q d.succ (prof.candidates.erase p.2)
           ( by rwa h_erase_card p.snd p2_in) (nat.succ_pos d)
       else false)
     with hvs,
   have viable_nonempty : viable_set.nonempty,
   { use ⟨a,b⟩,
     have : a ∈ (prof.candidates.erase b) := 
-      by simp only [mem_cands_of_mem_winners_new prof' a a_in],
-    simp only [simple_stable_voting_new, h_prof', h_erase_card b b_in, m_succ] at a_in,
+      by simp only [mem_cands_of_mem_winners prof' a a_in],
+    simp only [simple_stable_voting, h_prof', h_erase_card b b_in, m_succ] at a_in,
     simp only [finset.mem_filter, finset.mem_product, b_in, 
       dif_pos, dif_pos, and_true, finset.mem_filter, finset.mem_product],
     exact ⟨(finset.mem_erase.1 this).2, a_in⟩, },  
